devel/Iron/SystemF2Effect/Step/Preservation.v
@@ -1,33 +1,96 @@
 
 Require Export Iron.SystemF2Effect.Step.TfJudge.
 
+Fixpoint elem {A} (p : A -> bool) (xx : list A)
+ := match xx with
+    | nil      => false
+    | x :: xs  => if p x then true else elem p xs
+    end.
+
+
+Definition isSRegion (r : nat) (pp : stprop) : bool
+ := match pp with
+    | SRegion r' => beq_nat r r'
+    end.
+
+
+Definition hasSRegion (r : nat) (sp : stprops) 
+ := elem (isSRegion r) sp.
+
+
+Definition subsT_visible sp e e'
+ := SubsT e (maskOnCap (fun r => negb (hasSRegion r sp)) e').
+
+
+Lemma subsT_maskOnCap
+ :  forall p e1 e2
+ ,  SubsT e1 e2
+ -> SubsT e1 (maskOnCap p e2).
+Proof. admit. Qed.
+
+
+Lemma subsT_visible_refl
+ :  forall sp e
+ ,  subsT_visible sp e e.
+Proof.
+ intros.
+ unfold subsT_visible.
+  eapply subsT_maskOnCap.
+  auto.
+Qed.
+
+
+Lemma subsT_visible_equiv
+ :  forall sp e1 e2
+ ,  SubsT e1 e2
+ -> subsT_visible sp e1 e2.
+Proof.
+ intros.
+ unfold subsT_visible.
+  eapply subsT_maskOnCap.
+  auto.
+Qed.
+
+
+Lemma subsT_phase_change
+ :  forall sp p r e1 e2
+ ,  hasSRegion p sp = false
+ -> r               = TCap (TyCapRegion p)
+ -> SubsT e1 e2
+ -> subsT_visible sp e1 (liftTT 1 0 (substTT 0 r e2)).
+Proof.
+ admit.
+Qed.
+
 
 (* When a well typed expression transitions to the next state
    then its type is preserved. *)
 Theorem preservation
- :  forall se sp ss ss' fs fs' x x' t e
+ :  forall se sp sp' ss ss' fs fs' x x' t e
  ,  WfFS   se sp ss fs 
  -> TYPEC  nil nil se sp fs  x   t  e
- -> STEPF  ss  fs  x  ss' fs' x'
- -> (exists se' sp' e'
+ -> STEPF  ss  sp fs  x ss' sp' fs' x'
+ -> (exists se' e'
             ,  extends se' se
             /\ WfFS  se' sp' ss' fs'
-            /\ SubsT e e'
+            /\ subsT_visible sp e e'
             /\ TYPEC nil nil se' sp' fs' x' t e').
 Proof.
- intros se sp ss ss' fs fs' x x' t e HH HC HS. gen sp t e.
+ intros se sp sp' ss ss' fs fs' x x' t e.
+ intros HH HC HS. 
+ gen t e.
  induction HS; intros.
 
  (* Pure evaluation. *)
  Case "SfStep". 
  { inverts_typec. 
    exists se. 
-   exists sp. 
    exists e.
    rip.
-   eapply TcExp; eauto.
-   eapply stepp_preservation; eauto.
-   inverts HH. rip.
+   - apply subsT_visible_refl.
+   - eapply TcExp; eauto.
+     eapply stepp_preservation; eauto.
+     inverts HH. rip.
  }
 
  (* Push let context. *)
@@ -43,35 +106,44 @@ Proof.
  { inverts_typec.
    set (r := TCap (TyCapRegion p)).
    exists se.
-   exists (sp :> SRegion p).
    exists (TSum (substTT 0 r e0) (substTT 0 r e2)).
    rip.
 
    (* Effect of result is subsumed by previous. *)
-   eapply SbTrans.
-    eapply SbEquiv.
-    eapply EqSym. eauto.
-    eapply subsT_sum_merge.
-     
-     admit. (* TODO: handle phase change
-                     say result effect can't have any more actions on existing regions,
-                      but allow it to have effects on new regions.
-                     Get this by masking effects on fresh regions in result effect, 
-                      then checking that the original subsumes it.
-                    Change maskOnCap to take a predicate for this. *)
+   - eapply SbTrans.
+     + eapply SbEquiv.
+       eapply EqSym. eauto.
+     + simpl.
+       eapply subsT_sum_merge.
+       * have (substTT 0 r e0 = liftTT 1 0 (substTT 0 r e0)) by admit. (* no vars in subst result *)
+          rewrite H1. clear H1.
+         eapply subsT_phase_change with (p := p).
+          admit.                   (* ok, p not in sp, by goodness of allocRegionFs *)
+          subst r. auto.
+          admit.                   (* ok, e1 has no free vars *)
 
-     have HE2: (substTT 0 r e2 = e2) by admit.  (* e2 has no vars as under empty kienv *)
+       * have (substTT 0 r e2 = liftTT 1 0 (substTT 0 r e2)) by admit. (* no vars in subst result *)
+          rewrite H1. clear H1.
+         eapply subsT_phase_change with (p := p).
+          admit.                   (* ok, p not in sp, by goodness of allocRegionFs *)      
+          subst r.  auto.
+          auto.
+          
+   -  have HE2: (substTT 0 r e2 = e2) by admit.  (* e2 has no vars as under empty kienv *)
       rewrite HE2. auto.
 
    (* Result is well typed. *)
-   + eapply TcExp 
+     eapply TcExp 
        with (sp := sp :> SRegion p) 
             (t1 := substTT 0 r t0)
             (e1 := substTT 0 r e0)
             (e2 := substTT 0 r e2); auto.
 
+     (* Type of result is equivlent to before *)
+     + rewrite HE2. auto.
+
      (* Type is preserved after substituting region handle. *)
-     - have HTE: (nil = substTE 0 r nil).
+     + have HTE: (nil = substTE 0 r nil).
        rewrite HTE.
 
        have HSE: (se  = substTE 0 r se)
@@ -85,7 +157,7 @@ Proof.
        * subst r. auto.
 
      (* New frame stack is well typed. *)
-     - eapply TfConsUse.
+     + eapply TfConsUse.
        admit.            (* ok, region handle is fresh, goodness of allocRegionFs *)
        admit.            (* ok, t0 doesn't mention ^0 by lowerTT *)
  }
@@ -96,26 +168,26 @@ Proof.
 
    (* We can only pop if there is at least on region in the store. *)
    destruct sp.
+
    (* No regions in store. *)
-   + inverts HH. rip. 
+   - inverts HH. rip. 
      unfold STOREP in *.
      spec H4 p.
      have (In (FUse p) (fs :> FUse p)).
       inverts H4. rip. nope.
 
    (* At least one region in store. *)
-   + destruct s.
+   - destruct s.
      exists se.
-     exists (sp :> SRegion n).
      exists e2.
      rip.
-     - admit.  (* CHANGE to allow store well formed under smaller frame stack *)
+     + admit.  (* CHANGE to allow store well formed under smaller frame stack *)
 
      (* New effect subsumes old one. *)
-     - eauto. 
+     + eapply subsT_visible_equiv. eauto. 
 
      (* Resulting configuation is well typed. *)
-     - eapply TcExp 
+     + eapply TcExp 
          with (sp := sp :> SRegion n)
               (e1 := TBot KEffect)
               (e2 := e2); eauto.
